Adjust and complete nonregularity proof for a^nb^n

Game/FormalLanguages/BasicDefinitions.lean
@@ -15,15 +15,15 @@ instance : DecidableEq Symbol :=
 
 inductive Word where
   | ε
-  | cons (a : Symbol) (w : Word)
+  | cons (s : Symbol) (w : Word)
 
 def w₁ := Word.cons .a (Word.cons .b .ε)
 def w₂ := Word.cons .b (Word.cons .b (Word.cons .a .ε))
 
 @[simp]
-def Word.count (w : Word) (a : Symbol) : ℕ := match w with
+def Word.count (w : Word) (s' : Symbol) : ℕ := match w with
   | .ε => 0
-  | .cons s w => if (s = a) then 1 + w.count a else w.count a
+  | .cons s w => if (s = s') then 1 + w.count s' else w.count s'
 #reduce w₂.count .b
 
 theorem count_uneq (w u : Word) : (∃ (s : Symbol), w.count s ≠ u.count s) → w ≠ u := by
@@ -40,7 +40,7 @@ macro:max (priority := 1001) atomic("|" noWs) a:term noWs "|" : term => `(Word.l
 def Word.cat (x y : Word) : Word :=
   match x with
  | .ε => y
- | .cons a x => .cons a (x.cat y)
+ | .cons s x => .cons s (x.cat y)
 
 infixr:90 " ∘ " => Word.cat
 
@@ -50,9 +50,31 @@ lemma Word.cat_eps (w : Word) : w ∘ .ε = w := by
   · rw [cat]
   · rw [cat, ih]
 
+@[simp]
+lemma Word.cat_assoc (x y z : Word) : (x ∘ y) ∘ z = x ∘ y ∘ z := by
+  induction' x with s w ih <;> simp_all only [cat]
+
+@[simp]
+lemma Word.assoc_count {s : Symbol} (x y : Word) :
+    (x ∘ y).count s = x.count s + y.count s := by
+  induction' x with s' w ih
+  · simp_all only [cat, count, Nat.zero_add]
+  · rw [count]
+    simp_all only [cat, count]
+    split
+    next h =>
+      omega
+    next h => simp_all only
+
+@[simp]
+lemma Word.assoc_count_zero {s : Symbol} (x y : Word) :
+    (x ∘ y).count s = 0 → x.count s = 0 ∧ y.count s = 0 := by
+  intro hcatcount
+  apply And.intro <;> simp_all only [assoc_count, Nat.add_eq_zero_iff]
+
 lemma Word.cat_len (x y : Word) :
     |(x ∘ y)| = |x| + |y| := by
-  induction' x with a x ih
+  induction' x with s x ih
   · simp only [cat, length, Nat.zero_add]
   · rw [Word.length, Nat.add_assoc, ← ih]
     simp_all only [length]
@@ -80,11 +102,25 @@ infix:91 " ^+^ " => Symbol.pow
 lemma Symbol.pow_len {s : Symbol} (n : ℕ) : |s ^+^ n| = n := by
   induction' n with n ih
   · rfl
-  · simp only [Word.length]
+  · simp only [pow, Word.length]
     rw [ih]
     exact Nat.one_add _
 
+@[simp]
+lemma Symbol.pow_count {s₁ s₂ : Symbol} (n : ℕ) :
+    (s₁ ^+^ n).count s₂ = if s₁ = s₂ then n else 0 := by
+  induction' n with n ih
+  · simp_all only [pow, Word.count, ite_self]
+  · simp_all only [pow, Word.count, ↓reduceIte]
+    split
+    next h =>
+      subst h
+      simp_all only [↓reduceIte]
+      omega
+    next h => simp_all only [↓reduceIte]
+
 def anbn : Set Word := {w | ∃ n, w = .a ^+^ n ∘ .b ^+^ n}
+set_option linter.unusedVariables false
 
 @[simp]
 def pumping_property (L : Set Word) :=
@@ -94,7 +130,43 @@ def pumping_property (L : Set Word) :=
     ∃ (u v w : Word) (heq : z = u ∘ v ∘ w),
       |u ∘ v| ≤ n ∧
       |v| ≥ 1 ∧
-      ∀ (i : ℕ), u ∘ (v ^ i) ∘ w ∈ L
+      ∀ (i : ℕ), u ∘ v ^ i ∘ w ∈ L
+
+-- TODO: REFACTOR
+lemma Word.cons_a (n : ℕ) (x y z : Word) (hz : x ∘ y = .a ^+^ n ∘ z) (hx : |x| ≤ n) :
+    x.count .b = 0 := by
+  induction' x with s w ih generalizing n
+  · simp_all only [Word.length, Nat.zero_le, Word.count]
+  · specialize ih (n - 1)
+    simp_all only [Word.cat, Word.length, Word.count]
+    split
+    next h =>
+      subst h
+      simp_all only [Nat.add_eq_zero_iff, Nat.succ_ne_self, false_and]
+      match n with
+      | 0 =>
+        subst hz
+        simp_all only [Nat.le_zero_eq, Nat.add_eq_zero_iff, Nat.succ_ne_self, false_and]
+      | n + 1 =>
+        simp_all only [Nat.succ_sub_succ_eq_sub, Nat.sub_zero, cat, Nat.add_eq, Nat.add_zero,
+          cons.injEq, false_and]
+    next h =>
+      have ha : s = Symbol.a := by
+        match s with
+        | .a => rfl
+        | .b => exact False.elim (h rfl)
+      subst ha
+      match n with
+      | 0 =>
+        subst hz
+        simp_all only [not_false_eq_true, Nat.le_zero_eq, cat, Nat.zero_sub]
+        generalize length w = n at *
+        omega
+      | n + 1 =>
+        simp only [Nat.add_one_sub_one] at ih
+        rw [Symbol.pow] at hz
+        simp_all only [not_false_eq_true, cat, cons.injEq, true_and, forall_true_left]
+        exact ih (by omega)
 
 lemma not_pump : ¬pumping_property anbn := by
   rw [pumping_property]
@@ -125,13 +197,53 @@ lemma not_pump : ¬pumping_property anbn := by
         have hz : |z| = 2*n := by
           rw [heq, Word.cat_len, Symbol.pow_len, Symbol.pow_len]
           omega
-        sorry
+        simp_all only [gt_iff_lt, z]
+        have huv : (u ∘ v).count .b = 0 := by
+          symm at hcons
+          rw [← Word.cat_assoc] at hcons
+          apply Word.cons_a n (u ∘ v) w (.b ^+^ n) hcons hlenlower
+        exact (@Word.assoc_count_zero Symbol.b u v huv).right
       have hatleastonea : v.count .a > 0 := by
         clear hzinnonreg hlenlower hcons heq u w z hpos n
-        sorry
+        induction' v with s w ih
+        · simp_all only [Word.length, Nat.le_zero_eq, Nat.succ_ne_self]
+        · simp_all only [gt_iff_lt, Word.length, Nat.le_add_right, Word.count]
+          generalize w.count Symbol.a = n at *
+          split_ifs with hs
+          · subst hs
+            simp_all only [ite_false, forall_true_left]
+            have hsim : 1 ≤ 1 + n := by exact Nat.le_add_right 1 n
+            exact hsim
+          · split at honlyas
+            next h =>
+              subst h
+              simp_all only [Nat.add_eq_zero_iff, Nat.succ_ne_self, false_and]
+            next h =>
+              simp_all only [forall_const]
+              match s with
+              | .a => exact False.elim (hs rfl)
+              | .b => exact False.elim (h rfl)
       intro hin
       rw [anbn] at hin
       simp only [Word.pow, Word.cat_eps, Set.mem_setOf_eq] at hin
-      rcases hin with ⟨m, hm⟩
       --have h (w : Word) : w ∈ nonreg → w.count .a = w.count .b := sorry
-      sorry
+      simp_all only [gt_iff_lt, Word.cat_assoc, z]
+      have huneven : (u ∘ v ∘ v ∘ w).count .a ≠ (u ∘ v ∘ v ∘ w).count .b := by
+        simp only [Word.assoc_count, ne_eq, z]
+        apply Aesop.BuiltinRules.not_intro
+        intro heq
+        have hcount : (u ∘ v ∘ w).count .a = (u ∘ v ∘ w).count .b := by
+          rw [← hcons]
+          clear hcons
+          simp_all only [Nat.zero_add, Word.assoc_count, Symbol.pow_count, ite_true, ite_false,
+            Nat.add_zero]
+        simp only [Word.assoc_count] at hcount
+        have hgoal : v.count .a = v.count .b := by
+          omega
+        simp_all only [lt_self_iff_false, z]
+      rcases hin with ⟨m, hm⟩
+      have heven : (u ∘ v ∘ v ∘ w).count .a = (u ∘ v ∘ v ∘ w).count .b := by
+        clear huneven
+        simp_all only [Word.assoc_count, Symbol.pow_count, ite_true, ite_false, Nat.add_zero,
+          Nat.zero_add]
+      simp_all only [Word.assoc_count, ne_eq, z]
